Port AcceptOfMatch

RegexCorrectness/NFA/Basic.lean
@@ -52,3 +52,62 @@ theorem lt_of_inBounds_of_εStep {nfa : NFA} {i j : Nat} {h : i < nfa.nodes.size
       exact this.right
 
 end NFA
+
+namespace NFAa
+
+open NFA
+
+def εStep (nfa : NFAa) (i : Nat) : Set Nat :=
+  if h : i < nfa.nodes.size then
+    nfa[i].εStep
+  else ∅
+
+def charStep (nfa : NFAa) (i : Nat) (c : Char) : Set Nat :=
+  if h : i < nfa.nodes.size then
+    nfa[i].charStep c
+  else ∅
+
+-- def step (nfa : NFAa) (i : Fin nfa.nodes.size) (c : Option Char) : Set (Fin nfa.nodes.size) :=
+--   match c, nfa[i], nfa.inBounds i with
+--   | .some c, .char c' next, inBounds =>
+--     if c == c' then {⟨next, Node.lt_of_inBounds.char inBounds⟩} else ∅
+--   | .none, .epsilon next, inBounds => {⟨next, Node.lt_of_inBounds.epsilon inBounds⟩}
+--   | .none, .split next₁ next₂, inBounds =>
+--     have lt := Node.lt_of_inBounds.split inBounds
+--     {⟨next₁, lt.left⟩, ⟨next₂, lt.right⟩}
+--   | _, _, _ => ∅
+
+-- theorem charStep_cases {nfa : NFAa} {i j : Fin nfa.nodes.size} {c : Char}
+--   (h : j ∈ nfa.step i (.some c)) (char : nfa[i.val] = Node.char c j.val → motive)
+--   : motive := by
+--   simp [step] at h
+--   split at h <;> try simp [*] at *
+--   next c' c'' next _ eqn eqc _ =>
+--     apply char
+--     simp [eqn, eqc, h]
+
+-- theorem εStep_cases {nfa : NFAa} {i j : Fin nfa.nodes.size}
+--   (h : j ∈ nfa.step i .none)
+--   (epsilon : nfa[i.val] = Node.epsilon j.val → motive)
+--   (split : ∀ next₁ next₂, nfa[i.val] = Node.split next₁ next₂ → j.val = next₁ ∨ j.val = next₂ → motive) :
+--   motive := by
+--   simp [step] at h
+--   split at h <;> try simp [*] at *
+--   next next _ eqn _ _ =>
+--     apply epsilon
+--     simp [eqn, h]
+--   next next₁ next₂ _ eqn _ _ =>
+--     apply split next₁ next₂ eqn
+--     cases h <;> simp [*]
+
+-- theorem step_cases {nfa : NFAa} {i j : Fin nfa.nodes.size} (h : j ∈ nfa.step i c)
+--   (char : ∀ c', c = .some c' → nfa[i.val] = Node.char c' j.val → motive)
+--   (epsilon : c = none → nfa[i.val] = Node.epsilon j.val → motive)
+--   (split : ∀ next₁ next₂, c = none → nfa[i.val] = Node.split next₁ next₂ →
+--     j.val = next₁ ∨ j.val = next₂ → motive) :
+--   motive := by
+--   cases c with
+--   | none => apply εStep_cases h (epsilon rfl) (fun next₁ next₂ => split _ _ rfl)
+--   | some c' => apply charStep_cases h (char c' rfl)
+
+end NFAa
