RegexCorrectness/NFA/Compile.lean
@@ -512,7 +512,7 @@ namespace NFAa
 
 theorem pushRegex_get_lt (eq : pushRegex nfa next r = result) (i : Nat) (h : i < nfa.nodes.size) :
   result.val[i]'(Nat.lt_trans h result.property) = nfa[i] := by
-  induction r generalizing next nfa with
+  induction r generalizing nfa next with
   | empty | epsilon | char =>
     try apply pushRegex.empty eq
     try apply pushRegex.epsilon eq
@@ -557,5 +557,56 @@ theorem pushRegex_get_lt (eq : pushRegex nfa next r = result) (i : Nat) (h : i <
 
     have : nfa.nodes.size ≠ i := Nat.ne_of_gt h
     simp [this, ←get_eq_nodes_get, ih, eq₁, pushNode_get_lt _ h]
+
+theorem le_pushNode : nfa ≤ (pushNode nfa node h).val := by
+  intro i
+  have : i < (pushNode nfa node h).val.nodes.size := by
+    simp
+    exact Nat.lt_trans i.isLt (Nat.lt_succ_self _)
+  exists this
+  rw [pushNode_get_lt i i.isLt]
+
+theorem le_pushRegex : nfa ≤ (pushRegex nfa next r).val := by
+  induction r generalizing nfa next with
+  | empty | epsilon | char _ => unfold pushRegex; exact le_pushNode
+  | alternate r₁ r₂ ih₁ ih₂ =>
+    apply pushRegex.alternate (rfl : pushRegex nfa next (.alternate r₁ r₂) = _)
+    intro nfa₁ start₁ nfa₂ start₂ _ nfa' property eq₁ _ eq₃ _ eq₅ eq
+    rw [eq]
+
+    calc
+      _ ≤ nfa₁.val := eq₁ ▸ ih₁
+      _ ≤ nfa₂.val := eq₃ ▸ ih₂
+      _ ≤ nfa'.val := eq₅ ▸ le_pushNode
+  | concat r₁ r₂ ih₁ ih₂ =>
+    apply pushRegex.concat (rfl : pushRegex nfa next (.concat r₁ r₂) = _)
+    intro nfa₂ nfa₁ property eq₂ eq₁ eq
+    rw [eq]
+
+    calc
+      _ ≤ nfa₂.val := eq₂ ▸ ih₂
+      _ ≤ nfa₁.val := eq₁ ▸ ih₁
+  | star r ih =>
+    apply pushRegex.star (rfl : pushRegex nfa next (.star r) = _)
+    intro placeholder compiled patched nfa' isLt inBounds property
+      eq₁ eq₂ eq₃ eq₄ eq
+    rw [eq]
+
+    calc
+      _ ≤ placeholder.val := eq₁ ▸ le_pushNode
+      _ ≤ compiled.val := eq₂ ▸ ih
+      _ ≤ nfa' := by
+        intro i
+        have : i < nfa'.nodes.size := by
+          simp [eq₄, eq₃]
+        exists this
+        simp [eq₄, get_eq_nodes_get, eq₃]
+        rw [Array.get_set]
+        . split <;> try simp
+          next eqi =>
+            simp [←eqi, eq₂]
+            rw [←get_eq_nodes_get, pushRegex_get_lt rfl _ placeholder.property]
+            simp [eq₁]
+        . exact i.isLt
 
 end NFAa
