RegexCorrectness/NFA/Transition/AcceptOfMatch.lean
@@ -1,0 +1,455 @@
+-- When the regex matches a string, the compiled NFA accepts it.
+import RegexCorrectness.NFA.Basic
+import RegexCorrectness.NFA.Compile
+import RegexCorrectness.NFA.Order
+import RegexCorrectness.Lemmas
+
+import Mathlib.Data.Set.Basic
+import Mathlib.Data.Set.Lattice
+
+open Set
+
+namespace NFAa
+
+open NFA Node
+
+-- def lt_of_mem_of_εStep {nfa : NFAa} {i : Nat} {h : i < nfa.nodes.size} (mem : j ∈ nfa[i].εStep) :
+--   j < nfa.nodes.size := by
+--   have := nfa.inBounds ⟨i, h⟩
+--   simp at this
+--   simp [get_eq_nodes_get, εStep] at mem
+--   split at mem <;> try simp [*] at * <;> simp [Node.inBounds] at this
+--   . simp [mem, this]
+--   . cases mem <;> simp [*]
+
+theorem sub_εStep_of_le {nfa₁ nfa₂ : NFAa} (le : nfa₁ ≤ nfa₂) :
+  nfa₁.εStep i ⊆ nfa₂.εStep i := by
+  if h : i < nfa₁.nodes.size then
+    have : i < nfa₂.nodes.size := Nat.lt_of_lt_of_le h (le_size_of_le le)
+    simp [εStep, h, this]
+    obtain ⟨_, le⟩ := le ⟨i, h⟩
+    exact le.right
+  else
+    simp [εStep, h]
+
+theorem sub_charStep_of_le {nfa₁ nfa₂ : NFAa} (le : nfa₁ ≤ nfa₂) :
+  nfa₁.charStep i c ⊆ nfa₂.charStep i c := by
+  if h : i < nfa₁.nodes.size then
+    have : i < nfa₂.nodes.size := Nat.lt_of_lt_of_le h (le_size_of_le le)
+    simp [charStep, h, this]
+    obtain ⟨_, le⟩ := le ⟨i, h⟩
+    exact le.left c
+  else
+    simp [charStep, h]
+
+-- FIXME: I wanted to make this a claim about `Fin nfa.nodes.size`, but it's super cumbersome
+-- to cast between `Fin nfa₁.nodes.size` and `Fin nfa₂.nodes.size` given `nfa₁ ≤ nfa₂`.
+-- I should have avoided using NFA's ordering for proofs...
+inductive εClosure (nfa : NFAa) : Nat → Set Nat where
+  | base : nfa.εClosure i i
+  | step {i j k : Nat} (step : j ∈ nfa.εStep i) (rest : nfa.εClosure j k) :
+    nfa.εClosure i k
+
+-- theorem lt_of_εClosure_left {nfa : NFAa} {i j : Nat} (h : j ∈ nfa.εClosure i) :
+--   i < nfa.nodes.size := by
+--   cases h with
+--   | base h => exact h
+--   | step h => exact h
+
+-- theorem lt_of_εClosure_right {nfa : NFAa} {i j : Nat} (h : j ∈ nfa.εClosure i) :
+--   j < nfa.nodes.size := by
+--   induction h with
+--   | base h => exact h
+--   | step _ _ _ ih => exact ih
+
+theorem εClosure_of_le {nfa₁ nfa₂ : NFAa} (le : nfa₁ ≤ nfa₂) (h : j ∈ nfa₁.εClosure i) :
+  j ∈ nfa₂.εClosure i := by
+  induction h with
+  | base => exact .base
+  | step step _ ih => exact .step (mem_of_subset_of_mem (sub_εStep_of_le le) step) ih
+
+theorem εClosure_subset_of_le {nfa₁ nfa₂ : NFAa} (le : nfa₁ ≤ nfa₂) :
+  nfa₁.εClosure i ⊆ nfa₂.εClosure i := by
+  intro j h
+  exact εClosure_of_le le h
+
+theorem εClosure_snoc {nfa : NFAa} (cls : j ∈ nfa.εClosure i) (step : k ∈ nfa.εStep j) :
+  k ∈ nfa.εClosure i := by
+  induction cls with
+  | base => exact .step step .base
+  | step step' _ ih => exact εClosure.step step' (ih step)
+
+theorem εClosure_trans {nfa : NFAa} (h₁ : j ∈ nfa.εClosure i) (h₂ : k ∈ nfa.εClosure j) :
+  k ∈ nfa.εClosure i := by
+  induction h₁ with
+  | base => exact h₂
+  | step head _ ih => exact .step head (ih h₂)
+
+def εClosureSet (nfa : NFAa) (S : Set Nat) : Set Nat := ⋃ i ∈ S, nfa.εClosure i
+
+@[simp]
+theorem subset_εClosureSet {nfa : NFAa} : S ⊆ nfa.εClosureSet S := by
+  intro i mem
+  simp [εClosureSet]
+  refine ⟨i, mem, ?_⟩
+  exact .base
+
+@[simp]
+theorem εClosureSet_singleton_base {nfa : NFAa} : i ∈ nfa.εClosureSet {i} := by
+  simp [εClosureSet]
+  exact .base
+
+@[simp]
+theorem εClosureSet_singleton_step {nfa : NFAa} {i j : Nat}
+  (h : i < nfa.nodes.size) (mem : j ∈ nfa[i].εStep) : j ∈ nfa.εClosureSet {i} := by
+  simp [εClosureSet]
+  exact .step (by simp [h, mem, εStep]) .base
+
+@[simp]
+theorem εClosureSet_singleton {nfa : NFAa} {i j : Nat} (h : j ∈ nfa.εClosure i):
+  j ∈ nfa.εClosureSet {i} := by
+  apply mem_iUnion_of_mem i
+  simp [h]
+
+@[simp]
+theorem εClosureSet_empty {nfa : NFAa} : nfa.εClosureSet ∅ = ∅ := by
+  simp [εClosureSet]
+
+@[simp]
+theorem εClosureSet_univ {nfa : NFAa} : nfa.εClosureSet univ = univ :=
+  univ_subset_iff.mp subset_εClosureSet
+
+theorem εClosureSet_subset {nfa₁ nfa₂ : NFAa} (hn : nfa₁ ≤ nfa₂) (hs : S₁ ⊆ S₂) :
+  nfa₁.εClosureSet S₁ ⊆ nfa₂.εClosureSet S₂ := by
+  apply biUnion_mono hs
+  intro i _
+  exact εClosure_subset_of_le hn
+
+@[simp]
+theorem εClosureSet_idempotent {nfa : NFAa} : nfa.εClosureSet (nfa.εClosureSet S) = nfa.εClosureSet S := by
+  apply eq_of_subset_of_subset
+  . simp [subset_def]
+    intro k h
+    simp [mem_iUnion, εClosureSet] at h
+    let ⟨i, h, j, cls, cls'⟩ := h
+    exact mem_iUnion_of_mem i (mem_iUnion_of_mem h (εClosure_trans cls cls'))
+  . apply subset_εClosureSet
+
+theorem εClosureSet_iUnion_distrib {nfa : NFAa} {S : Set α} {f : α → Set Nat} :
+  nfa.εClosureSet (⋃ i ∈ S, f i) = ⋃ i ∈ S, nfa.εClosureSet (f i) := by
+  simp [εClosureSet]
+
+theorem εClosureSet_union_distrib {nfa : NFAa} {S₁ S₂ : Set Nat} :
+  nfa.εClosureSet (S₁ ∪ S₂) = nfa.εClosureSet S₁ ∪ nfa.εClosureSet S₂ := by
+  apply eq_of_subset_of_subset
+  . simp [subset_def]
+    intro j h
+    simp [εClosureSet] at *
+    let ⟨i, h, cls⟩ := h
+    cases h with
+    | inl h => exact .inl ⟨i, h, cls⟩
+    | inr h => exact .inr ⟨i, h, cls⟩
+  . simp [subset_def]
+    intro j h
+    simp [εClosureSet] at *
+    cases h with
+    | inl h =>
+      let ⟨i, h, cls⟩ := h
+      exact ⟨i, .inl h, cls⟩
+    | inr h =>
+      let ⟨i, h, cls⟩ := h
+      exact ⟨i, .inr h, cls⟩
+
+def stepSet (nfa : NFAa) (S : Set Nat) (c : Char) : Set Nat :=
+  ⋃ i ∈ S, nfa.εClosureSet (nfa.charStep i c)
+
+@[simp]
+def stepSet_empty {nfa : NFAa} : nfa.stepSet ∅ c = ∅ := by
+  simp [stepSet]
+
+@[simp]
+theorem εClosureSet_stepSet {nfa : NFAa} :
+  nfa.εClosureSet (nfa.stepSet S c) = nfa.stepSet S c := by
+  apply eq_of_subset_of_subset
+  . conv =>
+      lhs
+      simp [stepSet, εClosureSet_iUnion_distrib]
+  . exact subset_εClosureSet
+
+theorem stepSet_union_distrib {nfa : NFAa} {S₁ S₂ : Set Nat} :
+  nfa.stepSet (S₁ ∪ S₂) c = nfa.stepSet S₁ c ∪ nfa.stepSet S₂ c := by
+  simp [stepSet, εClosureSet_union_distrib]
+  apply eq_of_subset_of_subset
+  . intro j
+    simp
+    intro i mem cls
+    cases mem with
+    | inl mem => exact .inl ⟨i, mem, cls⟩
+    | inr mem => exact .inr ⟨i, mem, cls⟩
+  . intro j
+    simp
+    intro h
+    match h with
+    | .inl ⟨i, mem, cls⟩ => exact ⟨i, .inl mem, cls⟩
+    | .inr ⟨i, mem, cls⟩ => exact ⟨i, .inr mem, cls⟩
+
+theorem stepSet_insert_distrib {nfa : NFAa} :
+  nfa.stepSet (insert i S) c = nfa.stepSet S c ∪ nfa.stepSet {i} c := by
+  have : nfa.stepSet (S ∪ {i}) c =  nfa.stepSet S c ∪ nfa.stepSet {i} c :=
+    stepSet_union_distrib
+  simp at this
+  exact this
+
+theorem stepSet_subset {nfa₁ nfa₂ : NFAa} (hn : nfa₁ ≤ nfa₂) (hs : S₁ ⊆ S₂) :
+  nfa₁.stepSet S₁ c ⊆ nfa₂.stepSet S₂ c := by
+  simp [subset_def, stepSet]
+  intro j i h₁ h₂
+
+  exact ⟨
+    i,
+    mem_of_subset_of_mem hs h₁,
+    mem_of_subset_of_mem (εClosureSet_subset hn (sub_charStep_of_le hn)) h₂
+  ⟩
+
+theorem foldl_stepSet_subset_of_le {nfa₁ nfa₂ : NFAa} (le : nfa₁ ≤ nfa₂) (h : S₁ ⊆ S₂) :
+  List.foldl nfa₁.stepSet S₁ cs ⊆ List.foldl nfa₂.stepSet S₂ cs := by
+  induction cs generalizing S₁ S₂ with
+  | nil => simp [h]
+  | cons c _ ih =>
+    simp
+    apply ih
+    exact stepSet_subset le h
+
+theorem foldl_stepSet_subset {nfa : NFAa} (h : S₁ ⊆ S₂) :
+  List.foldl nfa.stepSet S₁ cs ⊆ List.foldl nfa.stepSet S₂ cs :=
+  foldl_stepSet_subset_of_le le_refl h
+
+theorem foldl_stepSet_iUnion_distrib {nfa : NFAa} {S : Set α} {f : α → Set Nat} :
+  List.foldl nfa.stepSet (⋃ i ∈ S, f i) cs = ⋃ i ∈ S, List.foldl nfa.stepSet (f i) cs := by
+  induction cs generalizing S f with
+  | nil => simp
+  | cons c _ ih => simp [stepSet, ih]
+
+theorem εClosureSet_subset_foldl_stepSet {nfa : NFAa} (h : S' ⊆ List.foldl nfa.stepSet (nfa.εClosureSet S) cs) :
+  nfa.εClosureSet S' ⊆ List.foldl nfa.stepSet (nfa.εClosureSet S) cs := by
+  induction cs generalizing S S' with
+  | nil =>
+    simp at *
+    calc nfa.εClosureSet S'
+      _ ⊆ nfa.εClosureSet (nfa.εClosureSet S) := εClosureSet_subset le_refl h
+      _ = nfa.εClosureSet S := εClosureSet_idempotent
+  | cons c _ ih =>
+    simp at *
+    simp [stepSet, ←εClosureSet_iUnion_distrib]
+    apply ih
+    apply Subset.trans h
+    apply foldl_stepSet_subset
+    simp [stepSet]
+    intro i hi j hj
+    simp [εClosureSet_iUnion_distrib]
+    exact ⟨i, hi, hj⟩
+
+def evalFrom (nfa : NFAa) (S : Set Nat) : List Char → Set Nat :=
+  List.foldl (nfa.stepSet) (nfa.εClosureSet S)
+
+theorem mem_evalFrom_subset {nfa : NFAa} (hmem : next ∈ nfa.evalFrom S₁ s) (hs : S₁ ⊆ nfa.εClosureSet S₂) :
+  next ∈ nfa.evalFrom S₂ s := by
+  apply mem_of_subset_of_mem _ hmem
+  apply le_foldl_of_le
+  . intro _ _ _ hs
+    exact stepSet_subset le_refl hs
+  . suffices nfa.εClosureSet S₁ ⊆ nfa.εClosureSet (nfa.εClosureSet S₂) by
+      simp at this
+      exact this
+    exact εClosureSet_subset le_refl hs
+
+theorem evalFrom_subset {nfa₁ nfa₂ : NFAa} {S₁ S₂ : Set Nat} (hn : nfa₁ ≤ nfa₂) (hs : S₁ ⊆ S₂) :
+  nfa₁.evalFrom S₁ s ⊆ nfa₂.evalFrom S₂ s := by
+  apply le_foldl_of_le
+  . intro _ _ _ hs
+    exact stepSet_subset hn hs
+  . exact εClosureSet_subset hn hs
+
+theorem mem_evalFrom_le {nfa₁ nfa₂ : NFAa} (le : nfa₁ ≤ nfa₂) (h : next ∈ nfa₁.evalFrom S s) :
+  next ∈ nfa₂.evalFrom S s :=
+  evalFrom_subset le Subset.rfl h
+
+-- Proof of the main result
+
+theorem evalFrom_of_matches.alternateLeft {s : String} (eq : pushRegex nfa next (.alternate r₁ r₂) = nfa')
+  (ih : ∀ {nfa next} {nfa'}, pushRegex nfa next r₁ = nfa' → ∀ (nfa'' : NFAa), nfa' ≤ nfa'' →
+    next.val ∈ nfa''.evalFrom {nfa'.val.start.val} s.data) :
+  next.val ∈ nfa'.val.evalFrom {nfa'.val.start.val} s.data := by
+  apply pushRegex.alternate eq
+  intro nfa₁ start₁ nfa₂ start₂ _ nfa' property eq₁ eq₂ eq₃ _ eq₅ eq
+  rw [eq]
+  simp
+  have := ih eq₁.symm nfa₁ le_refl
+  apply mem_of_mem_of_subset this
+  unfold evalFrom
+  have le : nfa₁.val ≤ nfa'.val :=
+    calc nfa₁.val
+      _ ≤ nfa₂.val := eq₃ ▸ le_pushRegex
+      _ ≤ nfa' := eq₅ ▸ le_pushNode
+  apply foldl_stepSet_subset_of_le le
+  calc nfa₁.val.εClosureSet {nfa₁.val.start.val}
+    _ ⊆ nfa'.val.εClosureSet {nfa₁.val.start.val} := εClosureSet_subset le Subset.rfl
+    _ ⊆ nfa'.val.εClosureSet {nfa'.val.start.val} := by
+      simp [εClosureSet]
+      intro i h
+      have mem : nfa₁.val.start.val ∈ nfa'.val.εClosure nfa'.val.start := by
+        rw [eq₅]
+        refine εClosure.step ?_ .base
+        simp [εStep, Node.εStep, eq₂]
+      exact εClosure_trans mem h
+
+theorem evalFrom_of_matches.alternateRight {s : String} (eq : pushRegex nfa next (.alternate r₁ r₂) = nfa')
+  (ih : ∀ {nfa next} {nfa'}, pushRegex nfa next r₂ = nfa' → ∀ (nfa'' : NFAa), nfa' ≤ nfa'' →
+    next.val ∈ nfa''.evalFrom {nfa'.val.start.val} s.data) :
+  next.val ∈ nfa'.val.evalFrom {nfa'.val.start.val} s.data := by
+  apply pushRegex.alternate eq
+  intro nfa₁ start₁ nfa₂ start₂ _ nfa' property _ _ eq₃ eq₄ eq₅ eq
+  rw [eq]
+  simp
+  have := ih eq₃.symm nfa₂ le_refl
+  apply mem_of_mem_of_subset this
+  unfold evalFrom
+  have le : nfa₂.val ≤ nfa'.val := eq₅ ▸ le_pushNode
+  apply foldl_stepSet_subset_of_le le
+  calc nfa₂.val.εClosureSet {nfa₂.val.start.val}
+    _ ⊆ nfa'.val.εClosureSet {nfa₂.val.start.val} := εClosureSet_subset le Subset.rfl
+    _ ⊆ nfa'.val.εClosureSet {nfa'.val.start.val} := by
+      simp [εClosureSet]
+      intro i h
+      have mem : nfa₂.val.start.val ∈ nfa'.val.εClosure nfa'.val.start := by
+        rw [eq₅]
+        refine εClosure.step ?_ .base
+        simp [εStep, Node.εStep, eq₄]
+      exact εClosure_trans mem h
+
+theorem evalFrom_of_matches.concat {s s₁ s₂ : String} (eq : pushRegex nfa next (.concat r₁ r₂) = nfa')
+  (eqs : s = s₁ ++ s₂)
+  (ih₁ : ∀ {nfa next} {nfa'}, pushRegex nfa next r₁ = nfa' → ∀ (nfa'' : NFAa), nfa' ≤ nfa'' →
+    next.val ∈ nfa''.evalFrom {nfa'.val.start.val} s₁.data)
+  (ih₂ : ∀ {nfa next} {nfa'}, pushRegex nfa next r₂ = nfa' → ∀ (nfa'' : NFAa), nfa' ≤ nfa'' →
+    next.val ∈ nfa''.evalFrom {nfa'.val.start.val} s₂.data) :
+  next.val ∈ nfa'.val.evalFrom {nfa'.val.start.val} s.data := by
+  apply pushRegex.concat eq
+  intro nfa₂ nfa₁ property eq₂ eq₁ eq
+  rw [eq]
+  simp
+  unfold evalFrom
+  simp [eqs]
+  apply mem_of_mem_of_subset (ih₂ eq₂.symm nfa₂ le_refl)
+  calc nfa₂.val.evalFrom {nfa₂.val.start.val} s₂.data
+    _ ⊆ nfa₁.val.evalFrom {nfa₂.val.start.val} s₂.data :=
+      evalFrom_subset (eq₁ ▸ le_pushRegex) Subset.rfl
+    _ ⊆ _ := by
+      unfold evalFrom
+      apply foldl_stepSet_subset_of_le le_refl
+      apply εClosureSet_subset_foldl_stepSet
+      simp
+      exact ih₁ eq₁.symm nfa₁ le_refl
+
+theorem evalFrom_of_matches.starConcat {s s₁ s₂ : String} (eq : pushRegex nfa next (.star r) = nfa')
+  (eqs : s = s₁ ++ s₂)
+  (ih₁ : ∀ {nfa next} {nfa'}, pushRegex nfa next r = nfa' → ∀ (nfa'' : NFAa), nfa' ≤ nfa'' →
+    next.val ∈ nfa''.evalFrom {nfa'.val.start.val} s₁.data)
+  (ih₂ : ∀ {nfa next} {nfa'}, pushRegex nfa next (.star r) = nfa' → ∀ (nfa'' : NFAa), nfa' ≤ nfa'' →
+    next.val ∈ nfa''.evalFrom {nfa'.val.start.val} s₂.data) :
+  next.val ∈ nfa'.val.evalFrom {nfa'.val.start.val} s.data := by
+  apply pushRegex.star eq
+  intro placeholder compiled patched nfa' isLt inBounds property
+    eq₁ eq₂ eq₃ eq₄ eq'
+  rw [eq']
+  simp [eqs, evalFrom]
+  have ih₂ := ih₂ eq nfa' (by simp [eq'])
+  unfold evalFrom at ih₂
+  apply mem_of_mem_of_subset ih₂
+  apply foldl_stepSet_subset_of_le le_refl
+  apply εClosureSet_subset_foldl_stepSet
+  rw [eq']
+  simp
+  have : compiled.val ≤ nfa' := by
+    intro i
+    have : i < nfa'.nodes.size := by
+      rw [eq₄]
+      simp [eq₃]
+    exists this
+    simp [eq₄, get_eq_nodes_get]
+    simp [eq₃, Array.get_set]
+    split
+    case inl eq =>
+      conv =>
+        lhs
+        simp [eq₂, ←eq, ←get_eq_nodes_get]
+        simp [pushRegex_get_lt rfl _ placeholder.property]
+      simp [eq₁]
+    case inr _ => simp
+  have ih₁ := ih₁ eq₂.symm nfa' this
+  simp [evalFrom] at ih₁
+  have : nfa'.start.val = nfa.nodes.size := by
+    rw [eq₄]
+  rw [this]
+  apply mem_of_mem_of_subset ih₁
+  apply foldl_stepSet_subset_of_le le_refl
+  simp [εClosureSet]
+  intro i h
+  apply εClosure_trans (.step ?_ .base) h
+  simp [eq₄, εStep, isLt, get_eq_nodes_get]
+  simp [eq₃]
+  rw [Array.get_set_eq]
+  simp [Node.εStep]
+
+theorem evalFrom_of_matches (eq : pushRegex nfa next r = nfa')
+  (m : r.matches s) :
+  ∀ nfa'' : NFAa, nfa' ≤ nfa'' → next.val ∈ nfa''.evalFrom {nfa'.val.start.val} s.data := by
+  induction m generalizing next nfa with
+  | @char s c eqs =>
+    intro nfa'' le
+    apply mem_evalFrom_le le
+    simp [eqs, evalFrom, stepSet]
+    refine ⟨nfa'.val.start.val, by simp, ?_⟩
+    simp [εClosureSet]
+    refine ⟨next.val, ?_, .base⟩
+    rw [←eq]
+    simp [charStep, pushRegex, Node.charStep]
+  | @epsilon s eqs =>
+    intro nfa'' le
+    apply mem_evalFrom_le le
+    simp [eqs, evalFrom, εClosureSet]
+    refine .step ?_ .base
+    rw [←eq]
+    simp [εStep, pushRegex, Node.εStep]
+  | alternateLeft _ ih =>
+    intro nfa'' le
+    apply mem_evalFrom_le le
+    exact evalFrom_of_matches.alternateLeft eq ih
+  | alternateRight _ ih =>
+    intro nfa'' le
+    apply mem_evalFrom_le le
+    exact evalFrom_of_matches.alternateRight eq ih
+  | concat s s₁ s₂ r₁ r₂ eqs _ _ ih₁ ih₂ =>
+    intro nfa'' le
+    apply mem_evalFrom_le le
+    exact evalFrom_of_matches.concat eq eqs ih₁ ih₂
+  | starEpsilon eqs =>
+    intro nfa'' le
+    apply mem_evalFrom_le le
+    apply pushRegex.star eq
+    intro placeholder compiled patched nfa' isLt inBounds property
+      _ _ eq₃ eq₄ eq
+    rw [eq, eqs]
+    simp [evalFrom, εClosureSet]
+    apply εClosure.step ?_ .base
+    rw [eq₄]
+    simp [εStep, isLt, get_eq_nodes_get]
+    simp [eq₃]
+    rw [Array.get_set_eq]
+    simp [Node.εStep]
+  | starConcat s s₁ s₂ r eqs _ _ ih₁ ih₂ =>
+    intro nfa'' le
+    apply mem_evalFrom_le le
+    exact evalFrom_of_matches.starConcat eq eqs ih₁ ih₂
+
+end NFAa
